@@ -1,19 +1,21 @@
 import Roolean.SmtLib2.Executor
 import Roolean.QfBv.Interpretation
 
-
-def load (filename: String): IO (Except EParser (Array SmtCommand)) := do
-  let byteArray ← IO.FS.readBinFile filename
-  let chars := byteArray.toList
-
-  pure (parse chars)
-
 def main : IO Unit := do
-  let commands ← load "benchmarks/lean.smt2"
+  let problem ← IO.FS.readBinFile "benchmarks/lean.smt2"
+  let proof ← IO.FS.readBinFile "benchmarks/lean.proof"
+
+  let proof ← match Proof.parse proof.toList with
+  | Except.ok proof => pure proof
+  | Except.error err =>
+    IO.println s!"Proof parsing error: {reprStr err}"
+    return
+
+  let commands := parse problem.toList
   match commands with
     | Except.ok commands =>
       -- IO.println s!"Parsed commands: {reprStr commands}"
-      let executed ← execute Interpretation commands
+      let executed ← execute Interpretation commands proof
       match executed with
         | Except.ok () =>
           IO.println s!"Execution successful"
@@ -22,6 +24,6 @@ def main : IO Unit := do
           IO.println s!"Execution error: {reprStr err}"
 
     | Except.error err =>
-      IO.println s!"Parser error: {reprStr err}"
+      IO.println s!"Problem parsing error: {reprStr err}"
 
 #eval main
